

\begin{equation}
    u(\xi,\eta) = R(\eta) u(\xi)
    \label{lr_eq:sbfem_disp_interpolation}
\end{equation}

\begin{equation}
    \epsilon(\xi,\eta) = Lu(\xi,\eta)
    \label{lr_eq:sbfem_strain_disp_relation}
\end{equation}

\begin{equation}
    L = b_1(\eta) \frac{\partial}{\partial \xi} +
        \frac{1}{\xi}b_2(\eta)
\end{equation}

\begin{equation}
    \begin{aligned}
    b_1(\eta) & = \frac{1}{|J|}
            \begin{bmatrix}
                y_b(\eta),_{\eta}   &   0   \\
                0   &   -x_b(\eta),_{\eta}  \\
                -x_b(\eta),_{\eta} & y_b(\eta),_{\eta}
            \end{bmatrix} \\
    b_2(\eta) & = \frac{1}{|J|}
            \begin{bmatrix}
                -y_b    &   0   \\
                0       &   x_b \\
                x_b     &   y_b
            \end{bmatrix}
    \end{aligned}
    \label{lr_eq:sbfem_little_b}
\end{equation}

\begin{equation}
    |J| = x_b(\eta)y_b(\eta),_{\eta}
        - y_b(\eta)x_b(\eta),_{\eta}
    \label{lr_eq:sbfem_Jdet}
\end{equation}

\begin{equation}
    \sigma(\xi,\eta) = DB_1(\eta)u(\xi),_{\xi} +
                        \frac{1}{\xi}DB_2(\eta)u(\xi)
    \label{lr_eq:sbfem_stress}
\end{equation}

\begin{equation}
    \begin{aligned}
        B_1(\eta) &= b_1(\eta)R(\eta)    \\
        B_2(\eta) &= b_2(\eta)R(\eta),_{\eta}
        \label{lr_eq:sbfem_captial_b}
    \end{aligned}
\end{equation}

\begin{equation}
    \begin{aligned}
        \delta u(\xi)^{T} \left(
            (E_0 \xi u(\xi),_{\xi}
            + E_1^T u(\xi))|_{\xi=1}
            - F
        \right) - \\
        \int_0^1 \delta u(\xi)^T\left(
            E_0 \xi^2 u(\xi),_{\xi\xi} + (E_0 + E_1^T - E_1) \xi u(\xi),_{\xi}
            - E_2 u(\xi)
        \right) d\xi = 0
    \end{aligned}
    \label{lr_eq:sbfem_virtual_work}
\end{equation}

\begin{equation}
    F = (E_0 \xi u(\xi),_{\xi} + E_1^T u(\xi))|_{\xi=1}
    \label{lr_eq:sbfem_nodal forces}
\end{equation}

\begin{equation}
    E_0 \xi^2 u(\xi),{\xi\xi} + (E_0 + E_1^T - E_1)\xi u(\xi),_{\xi} - E_2 u(\xi) = 0
    \label{lr_eq:sbfem_ODE}
\end{equation}

\begin{equation}
    \begin{aligned}
        E_0 &= \int_\eta B_1(\eta)^T DB_1(\eta)|J|d\eta \\
        E_1 &= \int_\eta B_2(\eta)^T DB_1(\eta)|J|d\eta \\
        E_2 &= \int_\eta B_2(\eta)^T DB_2(\eta)|J|d\eta
    \end{aligned}
    \label{lr_eq:sbfem_coe_matrix}
\end{equation}

\begin{equation}
    \chi = \left\{
        \begin{matrix}
            u(\xi)  \\
            q(\xi)
        \end{matrix}
    \right\}
    \label{lr_eq:sbfem_ODE_soltion}
\end{equation}


\begin{equation}
    q(\xi) = E_0 \xi u(\xi),_{\xi}
            + E_1^T u(\xi)
    \label{lr_eq:sbfem_internal_force}
\end{equation}

\begin{equation}
    F = q(\xi=1) = (E_0\xi u(\xi),_{\xi} + E_1^Tu(\xi))|_{\xi=1}
    \label{lr_eq:sbfem_boundary_nodal_force}
\end{equation}

\begin{equation}
    \xi \chi(\xi),_{\xi} = -Z\chi(\xi)
    \label{lr_eq:sbfem_1stODE}
\end{equation}

\begin{equation}
    Z = \begin{bmatrix}
        E_0^{-1} E_1^T    &  -E_0^{-1}   \\
        E_1 E_0^{-1} E_1^T - E_2    &   -E_1 E_0^{-1}
    \end{bmatrix}
    \label{lr_eq:sbfem_zmatrix}
\end{equation}

\begin{equation}
    Z \begin{bmatrix}
        \Phi_u \\
        \Phi_q
    \end{bmatrix} = \begin{bmatrix}
        \Phi_u  \\
        \Phi_q
    \end{bmatrix} \Lambda_n
    \label{lr_eq:sbfem_eigen_decomp}
\end{equation}

\begin{equation}
    u(\xi) = \Phi_u \xi^{-\Lambda_n} c
    \label{lr_eq:sbfem_general_sol_disp}
\end{equation}

\begin{equation}
    q(\xi) = \Phi_q \xi^{-\Lambda_n} c
    \label{lr_eq:sbfem_general_sol_str}
\end{equation}

\begin{equation}
    c = \Phi_u^{-1} u_b
    \label{lr_eq:sbfem_int_constant}
\end{equation}

\begin{equation}
    u(\xi,\eta) = R(\eta) \Phi_u \xi ^{-\Lambda_n} c
    \label{lr_eq:sbfem_displacement_field}
\end{equation}

\begin{equation}
    \sigma(\xi,\eta) = \Psi_\alpha (\eta) \xi^{-\Lambda_n - I} c
    \label{lr_eq:sbfem_stress_field}
\end{equation}

\begin{equation}
    \Psi_\alpha(\eta) = D(-B_1(\eta)\Phi_u \Lambda_n + B_2(\eta)\Phi_u)
    \label{lr_eq:sbfem_stress_mode}
\end{equation}

\begin{equation}
    F = \Phi_q \Phi_u^{-1} u_b
    \label{lr_eq:sbfem_kmat_previous}
\end{equation}

\begin{equation}
    K = \Phi_q \Phi_u^{-1}
    \label{lr_eq:sbfem_kmat}
\end{equation}

\begin{equation}
    E_0 \xi^2 u(\xi),_{\xi\xi} +
    (E_0 + E_1^T - E_1)\xi u(\xi),_{\xi} -
    E_2 u(\xi) + \omega^2 M_0 \xi^2 u(\xi) = 0
    \label{lr_eq:sbfem_dynamic}
\end{equation}

\begin{equation}
    M_0 = \int_\eta R^T \rho R|J| d\eta
    \label{lr_eq:sbfem_dynamic_mass}
\end{equation}

\begin{equation}
    (S(\omega)-E_1)E_0^{-1}
    (S(\omega)-E_1^T) - E_2 +
    \omega S(\omega),_\omega + \omega^2 M_0 = 0
    \label{lr_eq:sbfem_dynamic_1stODE}
\end{equation}

\begin{equation}
    F = S(\omega) u(\xi=1)
    \label{lr_eq:sbfem_dynamic_nodal_force}
\end{equation}

\begin{equation}
    S(\omega) = K - \omega^2 M + \omega^4 \left[
        R^{(1)}    
    \right]^{-1}
    \label{lr_eq:sbfem_dynamic_stiffness}
\end{equation}

\begin{equation}
    R^{(1)} = S_0^{(1)} - \omega^2 S_1^{(1)} + \omega^4 [R^{(2)}]^{-1}
    \label{lr_eq:sbfem_dynamic_R}
\end{equation}

% \begin{equation}

% \end{equation}